src/3d/Options.fsti
@@ -1,7 +1,6 @@
 module Options
+open HashingOptions
 open FStar.All
-
-type check_hashes_t = | NoHashes | WeakHashes | StrongHashes
 
 val display_usage : unit -> ML unit
 
@@ -29,6 +28,6 @@ val get_skip_makefiles : unit -> ML bool
 
 val get_no_everparse_h : unit -> ML bool
 
-val get_check_hashes : unit -> ML check_hashes_t
+val get_check_hashes : unit -> ML (option check_hashes_t)
 
 val get_save_hashes : unit -> ML bool
