src/3d/HashingOptions.fst
@@ -1,0 +1,8 @@
+module HashingOptions
+
+type check_hashes_t = | WeakHashes | StrongHashes | InplaceHashes
+
+let is_weak = function
+  | WeakHashes
+  | InplaceHashes -> true
+  | _ -> false
